

Question 5.

Consider the process

(1) $F_t = f(t) \cdot g(w_t)$. Show that

fol-lw:

(9)
$$dF_t = f'(t) g(w_t) dt + \frac{1}{2} f(t) g''(w_t) dt + f(t) g'(w_t) dw_t$$

! $F_t = f(t) \cdot g(w_t) \Rightarrow$ let

(2) $F_t = \underbrace{\varphi(w_t, t)}_{\text{case II}} = f(t) \cdot g(w_t) \quad \&$

(3) $\varphi(x, t) = f(t) \cdot g(x)$, then

we have for case II of Itô's Formula

(4)
$$dF_t = \left[\frac{\partial \varphi}{\partial t}(w_t, t) + \frac{1}{2} \frac{\partial^2 \varphi}{\partial x^2}(w_t, t) \right] dt + \frac{\partial \varphi}{\partial x}(w_t, t) dw_t$$

We need the ↓:

(5) $\frac{\partial \varphi}{\partial t}(x, t) = \frac{\partial}{\partial t} [f(t) \cdot g(x)] = f'(t) \cdot g(x)$

(6) $\frac{\partial \varphi}{\partial x}(x, t) = \frac{\partial}{\partial x} [f(t) \cdot g(x)] = f(t) \cdot g'(x) \quad \&$

① (7) $\frac{\partial^2 \varphi}{\partial x^2}(x, t) = f(t) \cdot g''(x)$, then putting (6)-(7) to (4):

$$(8) \quad dF_t = \left[f'(t) \cdot g(w_t) + \frac{1}{2} f(t) g'(w_t) \right] dt + f(t) \cdot g'(w_t) dw_t \quad \text{as desired}$$



(b) Using case II integration form of Itô's formula (or integrating \int_a^b (8) :)

$$(9) \quad \int_a^b dF_t = \int_a^b \left[f'(t) \cdot g(w_t) + \frac{1}{2} f(t) g'(w_t) \right] dt + \int_a^b f(t) \cdot g'(w_t) dw_t$$

Let's solve (9) for $\int_a^b f(t) \cdot g'(w_t) dw_t$ as


this is what we need to obtain :

$$(10) \quad \int_a^b f(t) g'(w_t) dw_t = F_t \Big|_a^b - \int_a^b f'(t) \cdot g(w_t) dt - \frac{1}{2} \int_a^b f(t) \cdot g'(w_t) dt$$

(2) but we know $F_t = f(t) \cdot g(w_t)$ so subbing it into (10):

yields

$$\begin{aligned}
 (11) \quad \int_a^b f(t) \cdot g'(w_t) dw_t &= \overbrace{f(t) \cdot g(w_t)}^{F_t} \Big|_a^b \\
 &\quad - \int_a^b f'(t) \cdot g(w_t) dt \\
 &\quad - \frac{1}{2} \int_a^b f(t) \cdot g'(w_t) dt
 \end{aligned}$$

as desired. 

(c) Find

$$(12) \quad \int_0^T \underbrace{e^{\frac{t}{2}}}_{f(t)} \underbrace{\cos w_t}_{g'(w_t)} dw_t = ?$$

, in (12), let

$$(13) \quad f(t) = e^{\frac{t}{2}} \quad \&$$

$$(14) \quad g'(w_t) = \cos(w_t),$$

then applying formula (11) in part (b)

gives the desired result:

(3)

$$f'(t) = \frac{1}{2} e^{\frac{t}{2}} \quad \text{and} \quad g(w_t) = \sin(w_t) \quad \text{and} \\ g''(w_t) = -\sin(w_t)$$

by (11)

$$\int_0^T \underbrace{e^{\frac{t}{2}}}_{f(t)} \underbrace{\cos(w_t)}_{g'(w_t)} dw_t = \left. e^{\frac{t}{2}} \cdot \sin(w_t) \right|_0^T$$

$$- \int_0^T \frac{1}{2} e^{\frac{t}{2}} \cdot \sin(w_t) dt = \underbrace{\frac{1}{2} \int_0^T e^{\frac{t}{2}} (-\sin(w_t)) dt}_{=0} \\ = \left. e^{\frac{t}{2}} \cdot \sin(w_t) \right|_{t=0}^{t=T} + 0$$

$$= e^{\frac{T}{2}} \sin(w_T) - e^0 \cdot \sin(w_0) =$$

$$= e^{\frac{T}{2}} \sin(w_T) - \sin(0)$$

$$= e^{\frac{T}{2}} \sin(w_T),$$

